updated fa2 test client/hook contracts

execution/tests/FA2TokenTests.v
@@ -1,14 +1,6 @@
-
-
-
-
 Module FA2ClientContract.
 From ConCert Require Import Blockchain LocalBlockchain FA2Token FA2Interface.
 From ConCert Require Import Serializable.
-From ConCert Require Import LocalBlockchainTests.
-From ConCert Require Import BoundedN.
-Require Import Extras.
-
 From Coq Require Import Morphisms.
 Require Import Monads.
 Require Import Extras.
@@ -16,25 +8,32 @@ Require Import Containers.
 Require Import Automation.
 From RecordUpdate Require Import RecordUpdate.
 From Coq Require Import List.
-Require Import Serializable.
-Require Import Blockchain.
 Require Import ZArith.
 Import ListNotations.
 Import RecordSetNotations.
 
 Section FA2Client.
 Context {BaseTypes : ChainBase}.
-(* Context {FA2ContractAddr : Address}. *)
 Set Primitive Projections.
 Set Nonrecursive Elimination Schemes.
 Open Scope N_scope.
 
 Inductive FA2ClientMsg :=
-  | Call_fa2_is_operator : is_operator_param -> FA2ClientMsg. 
+  | Call_fa2_is_operator : is_operator_param -> FA2ClientMsg 
+  | Call_fa2_balance_of_param : list balance_of_response -> FA2ClientMsg
+  | Call_fa2_total_supply_param : list total_supply_response -> FA2ClientMsg
+  | Call_fa2_metadata_callback : list token_metadata -> FA2ClientMsg
+  | Call_fa2_permissions_descriptor : permissions_descriptor -> FA2ClientMsg.
 
 Global Instance FA2ClientMsg_serializable : Serializable FA2ClientMsg :=
-  Derive Serializable FA2ClientMsg_rect <Call_fa2_is_operator>.
-Definition Msg := @FA2ReceiverMsg BaseTypes FA2ClientMsg _.
+  Derive Serializable FA2ClientMsg_rect <
+    Call_fa2_is_operator, 
+    Call_fa2_balance_of_param, 
+    Call_fa2_total_supply_param,
+    Call_fa2_metadata_callback,
+    Call_fa2_permissions_descriptor>.
+
+Definition ClientMsg := @FA2ReceiverMsg BaseTypes FA2ClientMsg _.
 
 Record State := 
   build_state {
@@ -54,41 +53,13 @@ Instance setup_settable : Settable _ :=
 
 Section Serialization.
 
-
 Global Instance setup_serializable : Serializable Setup :=
   Derive Serializable Setup_rect <build_setup>.
 
-(* Global Instance Msg_serializable' : Serializable (@FA2ReceiverMsg BaseTypes FA2ClientMsg) :=
-Derive Serializable (@FA2ReceiverMsg_rect BaseTypes FA2ClientMsg) <
-  (@receive_balance_of_param BaseTypes FA2ClientMsg), 
-  (@receive_total_supply_param BaseTypes FA2ClientMsg), 
-  (@receive_metadata_callback BaseTypes FA2ClientMsg), 
-  (@receive_is_operator BaseTypes FA2ClientMsg), 
-  (@transfer_hook  BaseTypes FA2ClientMsg), 
-  (@other_msg BaseTypes FA2ClientMsg)>. *)
-
-(* Global Instance Msg_serializable : Serializable FA2Client.Msg :=  @FA2Interface.FA2ReceiverMsg_serializable. *)
-(* Import Serializable.
-Ltac make_serializable eliminator ctors :=
-  let ser := make_serializer eliminator in
-  let elim_ty := type of eliminator in
-  let ty := get_ty_from_elim_ty elim_ty in
-  let deser := make_deserializer ctors ty in
-  exact
-    {| serialize := ser;
-       deserialize := deser;
-       deserialize_serialize :=
-         ltac:(intros []; repeat (cbn in *; try rewrite deserialize_serialize; auto)) |}.
-Global Program Instance msg_serializable : Serializable FA2CallerMsg :=
-{| serialize := serialize_sum;
-   deserialize := deserialize_sum
-|}.
-Next Obligation.
-intros. rewrite deserialize_serialize_sum. 
-reflexivity. Qed. *)
-
 Global Instance state_serializable : Serializable State :=
 	Derive Serializable State_rect <build_state>.
+
+Global Instance ClientMsg_serializable : Serializable ClientMsg := FA2Token.FA2ReceiverMsg_serializable.
 
 End Serialization.
   
@@ -103,7 +74,7 @@ Definition init (chain : Chain)
 Definition receive (chain : Chain)
 						 			 (ctx : ContractCallContext)
 									 (state : State)
-									 (maybe_msg : option FA2Client.Msg)
+									 (maybe_msg : option ClientMsg)
 									 : option (State * list ActionBody) :=
 	match maybe_msg with
   | Some (receive_is_operator is_op_response) => Some (state<| bit:= 42|>, [])
@@ -137,12 +108,165 @@ Lemma receive_proper :
   Proper (ChainEquiv ==> eq ==> eq ==> eq ==> eq) FA2Client.receive.
 Proof. repeat intro; solve_contract_proper. Qed.
 
-Definition contract : Contract Setup Msg State :=
+Definition contract : Contract FA2Client.Setup ClientMsg FA2Client.State :=
   build_contract FA2Client.init init_proper FA2Client.receive receive_proper.
 
 End FA2Client.
-
 End FA2ClientContract.
+
+Module FA2TransferHookContract.
+(* A contract which implements the transfer hook endpoint of FA2 *)
+(* Behavior is driven by a permission policy *)
+
+From ConCert Require Import Blockchain LocalBlockchain FA2Token FA2Interface.
+From ConCert Require Import Serializable.
+From Coq Require Import Morphisms.
+Require Import Monads.
+Require Import Extras.
+Require Import Containers.
+Require Import Automation.
+From RecordUpdate Require Import RecordUpdate.
+From Coq Require Import List.
+Require Import ZArith.
+Import ListNotations.
+Import RecordSetNotations.
+
+Section FA2TransferHook.
+Context {BaseTypes : ChainBase}.
+Set Primitive Projections.
+Set Nonrecursive Elimination Schemes.
+Open Scope N_scope.
+
+Inductive FA2TransferHookMsg :=
+  | set_permission_policy : permissions_descriptor -> FA2TransferHookMsg.
+
+Global Instance FA2TransferHookMsg_serializable : Serializable FA2TransferHookMsg :=
+  Derive Serializable FA2TransferHookMsg_rect <
+    set_permission_policy>.
+
+Definition Msg := @FA2TransferHook BaseTypes FA2TransferHookMsg _.
+
+Record State := 
+  build_state {
+    owner : Address;
+    fa2_caddr : Address;
+    policy : permissions_descriptor;
+}.
+
+Record Setup := 
+  build_setup {
+    fa2_caddr_ : Address;
+    policy_ : permissions_descriptor;
+}.
+
+Instance state_settable : Settable _ :=
+  settable! build_state <owner; fa2_caddr; policy>.
+Instance setup_settable : Settable _ :=
+  settable! build_setup <fa2_caddr_; policy_>.
+
+Section Serialization.
+
+Global Instance setup_serializable : Serializable Setup :=
+  Derive Serializable Setup_rect <build_setup>.
+
+Global Instance state_serializable : Serializable State :=
+	Derive Serializable State_rect <build_state>.
+
+End Serialization.
+  
+Definition init (chain : Chain)
+								(ctx : ContractCallContext)
+								(setup : Setup) : option State := 
+  Some {|
+    owner := ctx.(ctx_from);
+    fa2_caddr := setup.(fa2_caddr_);
+    policy := setup.(policy_);
+	|}.
+
+Definition returnIf (cond : bool) := if cond then None else Some tt.
+
+Definition check_transfer_permissions (tr : transfer_descriptor)
+                                      (operator : Address)
+                                      (state : State) 
+                                      : option unit :=
+  if (address_eqb tr.(transfer_descr_from_) operator)
+  then if (FA2Token.policy_disallows_self_transfer state.(policy))
+    then None 
+    else Some tt
+  else if (FA2Token.policy_disallows_operator_transfer state.(policy))
+    then None
+    else Some tt.
+
+(* called whenever this hook receives a transfer from the FA2 contract *)
+(* checks the permission policy, and if all transfers are valid, 
+   forwards the transfers to the 'msg_receive_hook_transfer' endpoint of the FA2 Contract *)
+Definition on_hook_receive_transfer (caller : Address)
+                                    (param : transfer_descriptor_param)
+                                    (state : State)
+                                    : option (list ActionBody) :=
+  do _ <- returnIf (negb (address_eqb caller state.(fa2_caddr))) ;
+  do _ <- returnIf (negb (address_eqb param.(transfer_descr_fa2) state.(fa2_caddr))) ;
+  let operator := param.(transfer_descr_operator) in
+  let check_transfer_iterator tr acc :=
+    do _ <- check_transfer_permissions tr operator state ;
+    Some tt in
+  (* check if all transfers satisfy the permission policy. If at least one does not, the whole operation fails *)
+  do _ <- fold_right check_transfer_iterator (Some tt) param.(transfer_descr_batch) ;
+  (* send out transfer action *)
+  let msg := serialize (msg_receive_hook_transfer param) in
+  ret [(act_call caller 0%Z msg)].
+
+Definition try_update_permission_policy (caller : Address)
+                                    (new_policy : permissions_descriptor)
+                                    (state : State)
+                                    : (option State) :=
+  do _ <- returnIf (negb (address_eqb caller state.(owner))) ;
+  ret (state<| policy := new_policy |>).
+
+Definition receive (chain : Chain)
+						 			 (ctx : ContractCallContext)
+									 (state : State)
+									 (maybe_msg : option Msg)
+                   : option (State * list ActionBody) :=
+  let sender := ctx.(ctx_from) in
+  let without_actions := option_map (fun new_state => (new_state, [])) in
+	let without_statechange := option_map (fun acts => (state, acts)) in
+  match maybe_msg with
+  | Some (transfer_hook param) => without_statechange (on_hook_receive_transfer sender param state)
+  | Some (hook_other_msg (set_permission_policy policy)) => without_actions (try_update_permission_policy sender policy state)
+  | _ => None 
+	end.
+
+Ltac solve_contract_proper :=
+  repeat
+    match goal with
+    | [|- ?x _  = ?x _] => unfold x
+    | [|- ?x _ _ = ?x _ _] => unfold x
+    | [|- ?x _ _ _ = ?x _ _ _] => unfold x
+    | [|- ?x _ _ _ _ = ?x _ _ _ _] => unfold x
+    | [|- ?x _ _ _ _ = ?x _ _ _ _] => unfold x
+    | [|- ?x _ _ _ _ _ = ?x _ _ _ _ _] => unfold x
+    | [|- Some _ = Some _] => f_equal
+    | [|- pair _ _ = pair _ _] => f_equal
+    | [|- (if ?x then _ else _) = (if ?x then _ else _)] => destruct x
+    | [|- match ?x with | _ => _ end = match ?x with | _ => _ end ] => destruct x
+    | [H: ChainEquiv _ _ |- _] => rewrite H in *
+    | _ => subst; auto
+    end.
+
+Lemma init_proper :
+  Proper (ChainEquiv ==> eq ==> eq ==> eq) FA2TransferHook.init.
+Proof. repeat intro; solve_contract_proper.	Qed.
+
+Lemma receive_proper :
+  Proper (ChainEquiv ==> eq ==> eq ==> eq ==> eq) FA2TransferHook.receive.
+Proof. repeat intro; solve_contract_proper. Qed.
+
+Definition contract : Contract Setup Msg State :=
+  build_contract FA2TransferHook.init init_proper FA2TransferHook.receive receive_proper.
+
+End FA2TransferHook.
+End FA2TransferHookContract.
 
 Global Set Warnings "-extraction-logical-axiom".
 Require Import ZArith Strings.String.
@@ -162,34 +286,43 @@ Import RecordSetNotations.
 Require Import Extras.
 
 From ConCert.Execution.QCTests Require Import 
-	ChainGens TestUtils ChainPrinters SerializablePrinters TraceGens FA2Printers.
+	ChainGens TestUtils ChainPrinters TraceGens FA2Printers SerializablePrinters.
 (* For monad notations *)
-(* From ExtLib.Structures Require Import Monads.
-Import MonadNotation. Open Scope monad_scope. *)
+From ExtLib.Structures Require Import Monads.
+Import MonadNotation. Open Scope monad_scope.
 From Coq Require Import List Int.
 Import BoundedN.Stdpp.
 Import LocalBlockchain.
 Import ListNotations.
 Close Scope address_scope.
 
-Section Printers.
+
+Definition LocalChainBase : ChainBase := ChainGens.LocalChainBase.
+Let BaseTypes := ChainGens.LocalChainBase.
+Import FA2ClientContract.
+Import FA2TransferHookContract.
+(* Section Printers. *)
 Local Open Scope string_scope.
 
 Instance showFA2ClientMsg : Show FA2ClientContract.FA2ClientMsg :=
 {|
 	show m := match m with
-						| FA2ClientContract.Call_fa2_is_operator param => "call_fa2_is_operator " ++ show param 
+            | FA2ClientContract.Call_fa2_is_operator param => "Call_fa2_is_operator " ++ show param 
+            | FA2ClientContract.Call_fa2_balance_of_param param => "Call_fa2_balance_of_param " ++ show param 
+            | FA2ClientContract.Call_fa2_total_supply_param param => "Call_fa2_total_supply_param param " ++ show param
+            | FA2ClientContract.Call_fa2_metadata_callback param => "Call_fa2_metadata_callback param " ++ show param
+            | FA2ClientContract.Call_fa2_permissions_descriptor param => "Call_fa2_permissions_descriptor param " ++ show param
 						end
 |}.
 
-Instance showFA2ClientContractMsg : Show FA2ClientContract.Msg :=
+Instance showFA2ClientContractMsg : Show FA2ClientContract.ClientMsg :=
 {|
 	show m := show m
 |}.
 
 Instance showFA2ClientState : Show FA2ClientContract.State :=
 {|
-  show t := "FA2ClientContractState{" 
+  show t := "FA2ClientState{" 
             ++ "fa2_caddr: " ++ show t.(FA2ClientContract.fa2_caddr) ++ sep 
             ++ "bit: " ++ show t.(FA2ClientContract.bit) 
             ++ "}"
@@ -197,23 +330,46 @@ Instance showFA2ClientState : Show FA2ClientContract.State :=
 
 Instance showFA2Setup : Show FA2ClientContract.Setup :=
 {|
-  show t := "FA2ClientContractSetup{" 
+  show t := "FA2ClientSetup{" 
             ++ "fa2_caddr_: " ++ show t.(FA2ClientContract.fa2_caddr_) 
             ++ "}"
 |}.
-       
+
+Instance showFA2TransferHookMsg : Show FA2TransferHookContract.FA2TransferHookMsg :=
+{|
+	show m := match m with
+            | FA2TransferHookContract.set_permission_policy param => "set_permission_policy " ++ show param 
+						end
+|}.
+
+Instance showFA2TransferHookContractState : Show FA2TransferHookContract.State :=
+{|
+  show t := "FA2TransferHookState{" 
+            ++ "fa2_caddr: " ++ show t.(FA2TransferHookContract.fa2_caddr) ++ sep 
+            ++ "policy: " ++ show t.(FA2TransferHookContract.policy) ++ sep 
+            ++ "owner: " ++ show t.(FA2TransferHookContract.owner) 
+            ++ "}"
+|}.
+
+Instance showFA2TransferHookContractSetup : Show FA2TransferHookContract.Setup :=
+{|
+  show t := "FA2TransferHookSetup{" 
+            ++ "fa2_caddr_: " ++ show t.(FA2TransferHookContract.fa2_caddr_) ++ sep 
+            ++ "policy_: " ++ show t.(FA2TransferHookContract.policy_) ++ sep 
+            ++ "}"
+|}.
+
 Close Scope string_scope.
-End Printers.
+(* End Printers. *)
 
 (* Notation "f 'o' g" := (compose f g) (at level 50). *)
 
-(* Definition LocalChainBase : ChainBase := ChainGens.LocalChainBase. *)
-(* Let BaseTypes := ChainGens.LocalChainBase. *)
+
 (* Instance BaseTypes : ChainBase := ChainGens.LocalChainBase. *)
 (** example policies *)
 
 (* the policy which allows only token owners to transfer their own tokens. *)
-Definition own_policy : permissions_descriptor := {|
+Definition policy_self_only : permissions_descriptor := {|
   descr_self := self_transfer_permitted;
   descr_operator := operator_transfer_denied;
   descr_sender := owner_no_op;
@@ -221,8 +377,17 @@ Definition own_policy : permissions_descriptor := {|
   descr_custom := None;
 |}.
 
+(* the policy which allows only operators to transfer tokens. *)
+Definition policy_operators_only : permissions_descriptor := {|
+  descr_self := self_transfer_denied;
+  descr_operator := operator_transfer_permitted;
+  descr_sender := owner_no_op;
+  descr_receiver := owner_no_op;
+  descr_custom := None;
+|}.
+
 (* non-transferable token (neither token owner, nor operators can transfer tokens. *)
-Definition own_policy1 : permissions_descriptor := {|
+Definition policy_no_transfers : permissions_descriptor := {|
   descr_self := self_transfer_denied;
   descr_operator := operator_transfer_denied;
   descr_sender := owner_no_op;
@@ -230,15 +395,38 @@ Definition own_policy1 : permissions_descriptor := {|
   descr_custom := None;
 |}.
 
-Definition token_setup := FA2Token.build_setup [] own_policy .
-Definition deploy_fa2token : @ActionBody Base := create_deployment 0 FA2Token.contract token_setup.
+(* the policy which allows both owners and operators to transfer tokens. *)
+Definition policy_all : permissions_descriptor := {|
+  descr_self := self_transfer_permitted;
+  descr_operator := operator_transfer_permitted;
+  descr_sender := owner_no_op;
+  descr_receiver := owner_no_op;
+  descr_custom := None;
+|}.
 
+Definition token_metadata_0 : token_metadata := {|
+  metadata_token_id := 0%N;
+  metadata_decimals := 8%N;
+|}.
+
+Definition token_setup : FA2Token.Setup := {|
+  setup_total_supply := [];
+  setup_tokens := FMap.add 0%N token_metadata_0 FMap.empty; 
+  initial_permission_policy := policy_all;
+|}.
+Definition deploy_fa2token : @ActionBody Base := create_deployment 0 FA2Token.contract token_setup.
 Definition token_contract_base_addr : Address := BoundedN.of_Z_const AddrSize 128%Z.
 
 Definition token_client_setup := FA2ClientContract.build_setup token_contract_base_addr.
 Definition deploy_fa2token_client : @ActionBody Base := create_deployment 0 FA2ClientContract.contract token_client_setup.
 Definition client_contract_addr : Address := BoundedN.of_Z_const AddrSize 129%Z.
 
+Definition fa2hook_setup : FA2TransferHookContract.Setup := {|
+  FA2TransferHookContract.fa2_caddr_ := token_contract_base_addr;
+  FA2TransferHookContract.policy_ := policy_self_only; 
+|}.
+Definition deploy_fa2hook := create_deployment 0 FA2TransferHookContract.contract fa2hook_setup.
+Definition fa2hook_contract_addr : Address := BoundedN.of_Z_const AddrSize 130%Z.
 
 Definition chain_with_token_deployed : LocalChain :=  
   unpack_option (my_add_block lc_initial 
@@ -247,15 +435,18 @@ Definition chain_with_token_deployed : LocalChain :=
     build_act creator (act_transfer person_2 10);
     build_act creator (act_transfer person_3 10);
     build_act creator deploy_fa2token;
-    build_act creator deploy_fa2token_client
+    build_act creator deploy_fa2token_client;
+    build_act creator deploy_fa2hook
   ]).
+
+Definition client_other_msg := @other_msg _ FA2ClientContract.FA2ClientMsg _.
 
 Definition call_client_is_op_act :=
   let params := Build_is_operator_param 
       (Build_operator_param zero_address zero_address all_tokens)
       (Build_callback is_operator_response) in 
-  let msg := other_msg (FA2ClientContract.Call_fa2_is_operator params) in
-  act_call client_contract_addr 0%Z (serialize FA2ClientContract.Msg _ msg).
+  let msg := client_other_msg (FA2ClientContract.Call_fa2_is_operator params) in
+  act_call client_contract_addr 0%Z (serialize FA2ClientContract.ClientMsg _ msg).
 
 Definition chain1 : LocalChain :=
   unpack_option (my_add_block chain_with_token_deployed 
@@ -274,17 +465,30 @@ Definition token_state lc :=
   | None => None
   end.
 Compute (client_state chain1).
-Compute (show (token_state chain1)).
+(* Compute (show (token_state chain1)). *)
 
-Definition gClientMsg : G FA2ClientContract.Msg := 
+Definition gClientMsg : G FA2ClientContract.ClientMsg := 
   let params := Build_is_operator_param 
     (Build_operator_param zero_address zero_address all_tokens)
     (Build_callback is_operator_response) in
-  returnGen (other_msg (FA2ClientContract.Call_fa2_is_operator params)).
+  returnGen (client_other_msg (FA2ClientContract.Call_fa2_is_operator params)).
+
+Definition gClientMsg' := 
+  let params := Build_is_operator_param 
+    (Build_operator_param zero_address zero_address all_tokens)
+    (Build_callback is_operator_response) in
+  returnGen params.
+
+Sample gClientMsg'.
+Sample (
+  msg <- gClientMsg';;
+  returnGen 1
+).
+
 Definition gClientAction := liftM (fun msg => 
   Some (
     build_act person_1 (
-      act_call token_contract_base_addr 0%Z (serialize FA2ClientContract.Msg _ msg)
+      act_call token_contract_base_addr 0%Z (serialize FA2ClientContract.ClientMsg _ msg)
     )
   )) gClientMsg.
 
@@ -297,6 +501,15 @@ Definition token_reachableFrom (lc : LocalChain) pf : Checker :=
 
 Definition token_reachableFrom_implies_reachable (lc : LocalChain) pf1 pf2 : Checker := 
   reachableFrom_implies_reachable lc (gFA2ChainTraceList 1) pf1 pf2.
+
+Sample gClientMsg.
+Sample (
+        msg <- gClientMsg;;
+        returnGen msg
+        ).
+Sample gClientAction.
+
+Sample (gFA2ChainTraceList 1 chain_with_token_deployed 4).
 
 
 
